Added BSTNode class, methods to implement and comparator function

proj/TreeSet.dfy
@@ -1,18 +1,22 @@
 // A datatype that stores a value of type T or Nil (no value) 
 datatype Option<T> = Nil | Some(value: T)
 
+// Function type for comparing elements
+type ComparatorFunction<!T> = (T) -> nat 
+
 // Represents a sorted set of elements of type T. 
-class {:autocontracts} SortedSet<T(==)> {
+class {:autocontracts} TreeSet<T(==)> {
 
   // Abstract state variable used for specification purposes only (set of elements in the sorted set).  
   ghost var elems : set<T>;
 
+   // Comparator function that it is passed to the tree set, so it can order its elements. 
+  const comp_func: ComparatorFunction<T>;
+
+  const initializer: nat -> T; // required by new T[]
+
   // Concrete state variable with internal representation (initially filled with Nil). 
   // TODO: ver representacao de uma BST
-
-  // Internal parameter, with initial size of sorted set.
-  const initialCapacity := 101;
-
 
 
   // Predicate that formalizes the class invariant.
@@ -22,8 +26,11 @@ class {:autocontracts} SortedSet<T(==)> {
   }
 
   // Receives the hash function to be used and initializes the set as empty.
-  constructor () {
-
+  constructor (comp_func: ComparatorFunction<T>) 
+    ensures elems == {}
+    ensures this.comp_func == comp_func
+  {
+    this.comp_func := comp_func;
   }
 
   // Inserts a new element x into the sorted set (binary search tree).
@@ -40,7 +47,13 @@ class {:autocontracts} SortedSet<T(==)> {
   // Checks if an element X is in the sorted set (binary search tree).
   method contains(x: T) returns (res: bool)
   {
-    return false;
+
+  }
+
+  // Returns an ordered sequence with all the elements of the sorted set (binary search tree).
+  method asSeq() returns (res: seq<T>)
+  {
+
   }
 }
 
